formic_site_duct/formic.apis.duct.dfy
@@ -5,23 +5,29 @@ module DuctApis {
     import opened DuctTools
 
     class Views {
+
         static method Endpoints() returns (all: AllApiEndpoints)
         {
             var catalog := new AllApiEndpoints();
+            var appDb := new Database();
 
             var formic_landing := new FormicLandingPage();
+            formic_landing.SetDb(appDb);
             var home := new ApiEndpoint("/", ReturnType.Content(""), formic_landing);
             catalog.Add(home);
 
             var login_page := new LoginChallengePage();
+            login_page.SetDb(appDb);
             var login := new ApiEndpoint("/login", ReturnType.ChallengeGoogle("/"), login_page);
             catalog.Add(login);
 
             var save_user_page := new SaveUserPage();
+            save_user_page.SetDb(appDb);
             var save_user := new ApiEndpoint("/save_user", ReturnType.Content(""), save_user_page);
             catalog.Add(save_user);
 
             var secure_page := new SecurePage();
+            secure_page.SetDb(appDb);
             var secure := new ApiEndpoint("/secure", ReturnType.Content(""), secure_page);
             catalog.Add(secure);
             
